FromAxioms/Algebra.lean
@@ -22,3 +22,4 @@ import FromAxioms.Algebra.Sylow
 import FromAxioms.Algebra.LinAlg
 import FromAxioms.Algebra.Ordered
 import FromAxioms.Algebra.TowerLaw
+import FromAxioms.Algebra.PointIdeal
